\documentclass{article}
\newcommand{\nm}{\begin{equation}}
\newcommand{\enm}{\end{equation}}
\newcommand{\nma}{\begin{align*}}
\newcommand{\enma}{\end{align*}}
\newcommand{\lp}{\left(}
\newcommand{\rp}{\right)}
\usepackage[utf8]{inputenc}
\usepackage{graphicx}
\usepackage{amssymb}
\usepackage{physics}
\title{statemech: expectation value of nj}
\author{seth iwan }
\date{march 2020}

\begin{document}
\maketitle
\section{boson}
goal is to derive $\expval{ n_j}  = \frac{1}{\exp(\mu-\epsilon)-1}$
\begin{align*}
\expval{n_j}&=\sum_{\{n_k\}}n_j P\{n_k\} \\
&= \sum_{\{n_k\}}n_j \exp{\sum_{\{n_k\}} \beta\lp\mu-\epsilon_k\rp n_k}\frac{1}{\sum_{\{n_k\}}\exp{\sum_{\{n_k\}} \beta\lp\mu-\epsilon_k\rp n_k}} \\
&=-\frac{1}{\beta}\pdv{\epsilon_k} \ln(\mathcal{Z})
\end{align*}
\nm
\expval{n_j}=-\frac{1}{\beta}\pdv{\epsilon_k} \ln(\mathcal{Z})
\enm
i got this be making use of the fact that $P\{n_k\}=\exp{\sum_{\{n_k\}} \beta\lp\mu-\epsilon_k\rp n_k}\frac{1}{\sum_{\{n_k\}}\exp{\sum_{\{n_k\}} \beta\lp\mu-\epsilon_k\rp n_k}}$ and the fact the $\frac{\pdv{x}y}{y}=\pdv{x}\ln(y)$.  Equation 1 wil be used for both the boson and fermion case. 
\begin{align*}
\mathcal{Z}&=\prod_{k=0}^{\infty}\frac{1}{1-\exp{\beta\lp\mu-\epsilon_k\rp}} \\
&\text{plug this into equation 1} \\
\expval{n_j}&=-\frac{1}{\beta}\pdv{\epsilon_k} \ln(\prod_{k=0}^{\infty}\frac{1}{1-\exp{\beta\lp\mu-\epsilon_k\rp}}) \\
                 &=\frac{1}{\beta}\pdv{\epsilon_k} \ln(\prod_{k=0}^{\infty}1-\exp{\beta\lp\mu-\epsilon_k\rp}) \\
                 &=\frac{1}{\beta}\frac{\prod_{k=0}^{\infty}\exp{\beta\lp\mu-\epsilon_k\rp}}{\prod_{k=0}^{\infty}\lp1-\exp{\beta\lp\mu-\epsilon_k\rp}\rp} \\
                 \text{which simplifies into } \\
                 & \boxed {=\frac{1}{\exp(-\beta\lp \mu-\epsilon\rp)-1}}
\end{align*}

\section{fermion}
very similar to boson except $\mathcal{Z}=\prod_{k=0}^{\infty}\lp1+\exp{\beta\lp\mu-\epsilon_k\rp}\rp$

\begin{align*}
\text{plug this into equation 1} \\
\expval{n_j}&=-\frac{1}{\beta}\pdv{\epsilon_k} \ln(\prod_{k=0}^{\infty}\lp1+\exp{\beta\lp\mu-\epsilon_k\rp}\rp) \\
                 &=\frac{1}{\beta}\frac{\prod_{k=0}^{\infty}\exp{\beta\lp\mu-\epsilon_k\rp}}{\prod_{k=0}^{\infty}\lp1+\exp{\beta\lp\mu-\epsilon_k\rp}\rp} \\
                 \text{which simplifies into } \\
                 & \boxed {=\frac{1}{\exp(-\beta\lp \mu-\epsilon\rp)+1}}
\end{align*}


\end{document}